\documentclass[12pt]{article}
\linespread{1}

\usepackage{amsmath}
\usepackage{amsthm}
\usepackage{amssymb}
\usepackage{graphicx}
\usepackage{listings}
\usepackage{tabularx}
\usepackage{framed}
\usepackage{verbatim}
\usepackage{float}
\usepackage{hyperref}
\usepackage{color}
\usepackage[toc,page]{appendix}
\usepackage{mathrsfs,mathtools,esint}

\hfuzz=2000pt 

%\usepackage{fullpage}

\hoffset  0 true in
\voffset   0 true pt
\textheight  9 true in
\textwidth  6 true in 
\oddsidemargin 0 true in
\topmargin 0 true in
\headsep  0 true in
\headheight  0 true in
\footskip   .5 true in

\newtheorem{Riemann}{Riemann Theorem}
\newcommand{\ds}{\displaystyle}
\renewcommand{\arraystretch}{1.5}


\title{Numerical Results: Multiple time stepping algorithms for explicit one-step exponential integrators} 
\author{} 
\date{\today } 

\begin{document}
\maketitle
\noindent
\section{Problem definition}
\emph{Goal of paper:} \\
Construct efficient (MTS) algorithms based on classes of explicit one-step exponential integrators.\\

\emph{What's desirable about these methods?}\\
\begin{itemize}
\item Application to exponential Rosenbrock methods
\item Do not require computation of starting values
\item Easy implementation of adaptive time step control
\item Avoid matrix functions
\item Order of accuracy up to four to be demonstrated
\end{itemize}

\noindent
\emph{Problem we're solving:}
\begin{equation} 
u'(t) = F(t,u(t)) = Au(t) + g(t,u(t)),  u(t_0) = u_0 \tag{1.1} \label{eq: 1.1}
\end{equation}
on the interval $t_0 \leq t \leq T$, where the vector field $F(t,u(t))$ can be decomposed into a linear stiff part $Au(t)$ and nonlinear nonstiff part $g(t,u(t))$. We consider the case where the stiff part is cheap to compute and the nonstiff part is expensive.

\subsection{MTS Algorithm for ETD Methods}
\begin{equation}
\hat{p}_{n,i}(\tau) = \sum_{j=1}^{i-1} \Bigg(\sum_{k=1}^{l_{ij}} \frac{\alpha_{ij}^{(k)}}{c_i^kh^{k-1}(k-1)!}\tau^{k-1}\Bigg)g(t_n + c_jh,\hat{U}_{n,j}),
\tag{3.19a} \label{eq: 3.19a}
\end{equation}
\begin{equation}
\hat{q}_{n,s}(\tau) = \sum_{i=1}^{s} \Bigg(\sum_{k=1}^{m_i} \frac{\beta_{i}^{(k)}}{h^{k-1}(k-1)!}\tau^{k-1}\Bigg)g(t_n + c_ih,\hat{U}_{n,i}),
\tag{3.19b} \label{eq: 3.19b}
\end{equation}
To get $\hat{u}_{n+1}$ solve: 
\begin{equation}
y'_{n,i}(\tau) = Ay_{n,i}(\tau) + \hat{p}_{n,i}(\tau), \hspace{0.3cm} y_{n,i}(0) = \hat{u}_n \hspace{0.3cm} (2\leq i \leq s)
\tag{3.20} \label{eq: 3.20}
\end{equation}
\subsubsection{Strategy for computing $\hat{U}_{n,i}$}
\begin{enumerate}
\item Set $\hat{U}_{n,1} = \hat{u}_n$.
\item $\hat{U}_{n,1}$ is now known. Evaluate $\hat{p}_{n,2}(\tau)$ from (\ref{eq: 3.19a}) and solve (\ref{eq: 3.20}) with $i=2$ to obtain $\hat{U}_{n,2} \approx \hat{y}_{n,2}(c_2h)$.
\item $\hat{U}_{n,1}, \hat{U}_{n,2} $ is now known. Evaluate $\hat{p}_{n,3}(\tau)$ from (\ref{eq: 3.19a}) and solve (\ref{eq: 3.20}) with $i=3$ to obtain $\hat{U}_{n,3} \approx \hat{y}_{n,3}(c_3h)$.\\
$\vdots$
\item $\hat{U}_{n,1},\cdots \hat{U}_{n,s-1} $ is now known. Evaluate $\hat{p}_{n,s}(\tau)$ from (\ref{eq: 3.19a}) and solve (\ref{eq: 3.20}) with $i=s$ to obtain $\hat{U}_{n,s} \approx \hat{y}_{n,s}(c_sh)$.
\end{enumerate}

\begin{equation}
y'_{n}(\tau) = Ay_{n}(\tau) + \hat{q}_{n}(\tau), \hspace{0.3cm} y_{n}(0) = \hat{u}_n 
\tag{3.21} \label{eq: 3.21}
\end{equation}
\section{Numerical Algorithms} 
\subsection{A third order method \texttt{expRK32}} 
Consider the three stage ETD method of stiff order three with the following Butcher tableau.
\begin{center}
\begin{table}[h!]
\begin{tabular}{r|c c c}
$0$ &  &  &  \\
$c_2$ & $c_2\varphi_{1,2}$ &  \\
$\frac{2}{3}$ & $\frac{2}{3}\varphi_{1,3} - \frac{4}{9c_2}\varphi_{2,3}$ & $\frac{4}{9c_2}\varphi_{2,3}$\\
\hline 
 & $\varphi_1 - \frac{3}{2}\varphi_2 $ & $0$ & $\frac{3}{2}\varphi_2$\\
 & $\varphi_1$ & $\frac{3}{3c_2 - 2}\varphi_2$ & $\frac{3}{2 - 3c_2}\varphi_2$ 
\end{tabular}
\end{table}
\end{center}

From the Butcher tableau, \\
$l_{21} = q_1 = 1$,\\
$l_{31} = l_{32} = m_1 = m_3 = q_2 = q_3 = 2$,\\
$\alpha_{21}^{(1)} = c_2 , \alpha_{31}^{(1)} = \frac{2}{3}, \alpha_{32}^{(1)} = 0$,\\
$\beta_1^{(1)} = 1, \beta_1^{(2)} = -\frac{3}{2}, \beta_2^{(k)} = 0 \hspace{.2cm} \forall k = 1,...,m_2$,\\
$\beta_3^{(1)} = 0, \beta_3^{(2)} = \frac{3}{2}$,\\ 
$\bar{\beta}_2^{(1)} = \bar{\beta}_3^{(1)} = 0$,\\
$\bar{\beta}_2^{(2)} = -\bar{\beta}_3^{(2)} = \frac{3}{3c_2 - 2} (c_2 \neq \frac{2}{3})$.\\

We then have:
\begin{equation}
\hat{p}_{n,2}(\tau) = g(t_n,\hat{u}_n), \tag{3.30a} \label{eq: 3.30a}
\end{equation}
\begin{equation}
\hat{p}_{n,3}(\tau) = \frac{1}{c_2h}g(t_n + c_2h,\hat{U}_{n,2})\tau + (1- \frac{\tau}{c_2h})\hat{p}_{n,2}(\tau), \tag{3.30b} \label{eq: 3.30b}
\end{equation}
 \begin{equation}
 \hat{q}_{n,3}(\tau) = \frac{3}{2h}g(t_n + \frac{2}{3}h, \hat{U}_{n,3}) \tau + (1 - \frac{3\tau}{2h})\hat{p}_{n,2}(\tau), \tag{3.30c} \label{eq: 3.30c}
 \end{equation}
 \begin{equation}
 \hat{\bar{q}}_{n,3}(\tau) = \frac{3}{(3c_2-2)h}(g(t_n + c_2h,\hat{U}_{n,2}) - g(t_n + \frac{2}{3}h, \hat{U}_{n,3}) )\tau + \hat{p}_{n,2}(\tau). \tag{3.30c} \label{eq: 3.30d}
 \end{equation}
 

%________________________________________________________________________________%
%_________________________Another 3rd order method_______________________________%
\subsection{Third order method \texttt{expRK32s3}}
\begin{center}
\begin{tabular}{r|c c c}
$c_1 =0$ & & & \\
$c_2 \neq \frac{2}{3}$ & $c_2\varphi_{1,2}$ & & \\
$c_3 = \frac{2}{3}$& $\frac{2}{3}\varphi_{1,3} - \frac{4}{9c_2}\varphi_{2,3}$ & $\frac{4}{9c_2}\varphi_{2,3}$ & \\
\hline
& $b_1 = \varphi_1 - b_2-b_3$ & $b_2 = \frac{-2}{3c_2(c_2 - \frac{2}{3})}\varphi_2 + \frac{2}{c_2(c_2 - \frac{2}{3})}\varphi_3$ & $b_3 = \frac{c_2}{\frac{2}{3}(c_2 - \frac{2}{3})}\varphi_2 -\frac{2}{\frac{2}{3}(c_2 - \frac{2}{3})}\varphi_3$ \\
& $\bar{b}_1 = \varphi_1 - \bar{b}_2 - \bar{b}_3$ & $\bar{b}_2 = \frac{-2}{3c_2(c_2 - \frac{2}{3})}\varphi_2$ & $\bar{b}_3 = \frac{c_2}{\frac{2}{3}(c_2 - \frac{2}{3})}\varphi_2$ 
\end{tabular}
\end{center}
Note : $\varphi_{i,j} = \varphi_i(c_jhA)$  ,  $b_i = b_i(hA)$.\\
\underline{\textbf{Polynomials}}\\
Let \begin{equation} D_{n,i} = g(t_n + c_ih,\hat{U}_{n,i}) - g(t_n,\hat{u}_n).
\end{equation}
\begin{equation}
\hat{p}_{n,2}(\tau) = g(t_n,\hat{u}_n)
\end{equation}

\begin{equation}
\hat{p}_{n,3}(\tau) = g(t_n,\hat{u}_n) + \frac{4}{9c_2} \frac{\tau}{c_3^2h}D_{n,2}
\end{equation}

\begin{equation}
\hat{q}_{n,3}(\tau) = g(t_n,\hat{u}_n) + \frac{\tau}{h} \Bigg( \frac{-2}{3c_2(c_2 - \frac{2}{3})}D_{n,2} + \frac{c_2}{\frac{2}{3}(c_2 - \frac{2}{3})}D_{n,3} \Bigg) + \frac{\tau^2}{2h^2}\Bigg(\frac{2}{c_2(c_2-\frac{2}{3})}D_{n,2} - \frac{2}{\frac{2}{3}(c_2 - \frac{2}{3})}D_{n,3} \Bigg)
\end{equation}

\begin{equation}
\hat{\bar{q}}_{n,3}(\tau) = g(t_n,\hat{u}_n) + \frac{\tau}{h} \Bigg(\frac{-2}{3c_2(c_2 - \frac{2}{3})}D_{n,2} + \frac{c_2}{\frac{2}{3}(c_2 - \frac{2}{3})}D_{n,3}\Bigg)
\end{equation}

%_________________________4th order method_______________________________________%
\subsection{Fourth order method \texttt{expRK43s6}}
\begin{center}
\begin{table}[h!]
\begin{tabularx}{19cm}{r|c| X| X| X |X}
$0$ &  &  & & &\\
$c_2$ &  & & & &\\
$c_3$ & $a_{32} = \frac{c_3^2}{c_2}\varphi_{2,3}$ &  & & &\\
$c_4$ &$a_{42} = \frac{c_4^2}{c_2}\varphi_{2,4}$& $a_{4,3} = 0$& & &\\
$c_5$ & $a_{52} = 0$ & $a_{53} = \frac{-c_4c_5^2}{c_3(c_3-c_4)}\varphi_{2,5} + \frac{2c_5^3}{c_3(c_3-c_4)}\varphi_{3,5}$ & $a_{54} = \frac{c_3c_5^2}{c_4(c_3-c_4)}\varphi_{2,5} - \frac{2c_5^3}{c_4(c_3-c_4)}\varphi_{3,5}$ & & \\
$c_6$ & $a_{62} = 0$ & $a_{63} = \frac{-c_4c_6^2}{c_3(c_3-c_4)}\varphi_{2,6} + \frac{2c_6^3}{c_3(c_3-c_4)}\varphi_{3,6}$ & $a_{64} = \frac{c_3c_6^2}{c_4(c_3-c_4)}\varphi_{2,6} + \frac{2c_6^3}{c_4(c_3-c_4)}\varphi_{3,6}$ & $a_{65} =0$ & \\
\hline 
 & $b_2 = 0$ & $b_3 = 0$ & $b_4 = 0$& $b_5 = \frac{-c_6}{c_5(c_5-c_6)}\varphi_2 + \frac{2}{c_5(c_5-c_6)}\varphi_3$ & $b_6 =\frac{c_5}{c_6(c_5-c_6)}\varphi_2 - \frac{2}{c_6(c_5-c_6)}\varphi_3$\\
 & $\bar{b}_2 = 0$ & $\bar{b}_3 = \frac{-c_4}{c_3(c_3-c_4)}\varphi_2 + \frac{2}{c_3(c_3-c_4)}\varphi_3$ & $\bar{b}_4 = \frac{c_3}{c_4(c_3-c_4)}\varphi_2 - \frac{2}{c_4(c_3-c_4)}\varphi_3$& $\bar{b}_5 = 0$ & $\bar{b}_6 = 0$ 
\end{tabularx}
\end{table}
\end{center}
Conditions to be satisfied: $c_3 \neq c_4, c_5\neq c_6, c_6 \neq \frac{2}{3}, c_5 = \frac{4c_6 -3}{6c_6 -4}.$\\
Two sets of c values: 
\begin{itemize}
\item $c_2 = \frac{1}{2} = c_3 = c_5 ; c_4 = \frac{1}{3} ; c_6 = 1.$
\item $c_2 = c_3 = \frac{1}{2}; c_4 = c_6 = \frac{1}{3} ; c_5 = \frac{5}{6}.$
\end{itemize}

\underline{\textbf{Polynomials}}
\begin{equation}
\hat{p}_{n,2}(\tau) = g(t_n,\hat{u}_n)
\end{equation}

\begin{equation}
\hat{p}_{n,3}(\tau) = g(t_n,\hat{u}_n) + \frac{\tau}{c_2h}D_{n,2}
\end{equation}

\begin{equation}
\hat{p}_{n,4}(\tau) = g(t_n,\hat{u}_n) + \frac{\tau}{c_2h}D_{n,2}
\end{equation}

\begin{equation}
\hat{p}_{n,5}(\tau) = g(t_n,\hat{u}_n) + \frac{\tau}{h}\Bigg(\frac{-c_4}{c_3(c_3 - c_4)}D_{n,3} + \frac{c_3}{c_4(c_3 - c_4)}D_{n,4} \Bigg) + \frac{\tau^2}{2h^2}\Bigg(\frac{2}{c_3(c_3-c_4)}D_{n,3} - \frac{2}{c_4(c_3 - c_4)}D_{n,4} \Bigg)
\end{equation}

\begin{equation}
\hat{p}_{n,6}(\tau) = g(t_n,\hat{u}_n) + \frac{\tau}{h}\Bigg(\frac{-c_4}{c_3(c_3 - c_4)}D_{n,3} + \frac{c_3}{c_4(c_3 - c_4)}D_{n,4} \Bigg) + \frac{\tau^2}{2h^2}\Bigg(\frac{2}{c_3(c_3-c_4)}D_{n,3} - \frac{2}{c_4(c_3 - c_4)}D_{n,4} \Bigg)
\end{equation}

\begin{equation}
\hat{q}_{n,6}(\tau) = g(t_n,\hat{u}_n) + \frac{\tau}{h}\Bigg(\frac{-c_6}{c_5(c_5 - c_6)}D_{n,5} + \frac{c_5}{c_6(c_5 - c_6)}D_{n,6} \Bigg) + \frac{\tau^2}{2h^2}\Bigg(\frac{2}{c_5(c_5-c_6)}D_{n,5} - \frac{2}{c_6(c_5 - c_6)}D_{n,6} \Bigg)
\end{equation}

\begin{equation}
\hat{\bar{q}}_{n,6}(\tau) = g(t_n,\hat{u}_n) + \frac{\tau}{h}\Bigg(\frac{-c_4}{c_3(c_3 - c_4)}D_{n,3} + \frac{c_3}{c_4(c_3 - c_4)}D_{n,4} \Bigg) + \frac{\tau^2}{2h^2}\Bigg(\frac{2}{c_3(c_3-c_4)}D_{n,3} - \frac{2}{c_4(c_3 - c_4)}D_{n,4} \Bigg)
\end{equation}

\section{Test problems}
%_____________________________________________________________________________%
%________________________Brusselator Problem__________________________________%
%_____________________________________________________________________________%
\subsection{Brusselator Problem}
We consider the Brusselator problem represented by  \emph{(Why?)}
\begin{equation}
\mathbf{\frac{dy}{dt}} = \begin{bmatrix}
a - (y_3 + 1)y_1 + y_1^2y_2\\ y_3y_1 - y_1^2y_2\\ \frac{b-y_3}{\epsilon} - y_1y_3
\end{bmatrix}
\end{equation}
This equation in the form of (\ref{eq: 1.1}) becomes
\begin{equation}
\mathbf{\frac{dy}{dt}} = \begin{bmatrix}
0 & 0 & 0 \\ 0 & 0 & 0 \\ \frac{-1}{\epsilon} & 0 & 0
\end{bmatrix} \begin{bmatrix}
y_1 \\ y_2 \\ y_3
\end{bmatrix}  + \begin{bmatrix}
a - (y_3 + 1)y_1 + y_1^2y_2\\ y_3y_1 - y_1^2y_2\\ \frac{b}{\epsilon} - y_1y_3
\end{bmatrix}
\end{equation}
where $y_1(0) = 1.2, y_2(0) = 3.1,$ and $y_3(0) = 3$, with parameters $a=1, b=3.5,$ and $\epsilon =0.01$.  We evaluate over the time interval $[0,10]$. We investigate the performance of the algorithm when ODE solvers of different orders are used for the inner steps. For each ODE solver, the macro time steps are given by the $h-$values and $h/m$ determines the micro time steps.\\

%_______________________________________________________________________%
%__________________________Prothero-Robinson____________________________%
\subsection{Modified Prothero-Robinson Problem}
We consider the Modified Prothero-Robinson Problem
\begin{equation}
\mathbf{\frac{dy}{dt}} = \begin{bmatrix}
\Gamma & \epsilon \\ \epsilon & 1
\end{bmatrix}    \begin{bmatrix} y_1 - g(t) \\ y_2 - g(\omega t) \end{bmatrix} - \begin{bmatrix}
g(t) \\ g(\omega t)
\end{bmatrix}' 
\end{equation}
In the form of (\ref{eq: 1.1}) we have \begin{equation}
\mathbf{\frac{dy}{dt}} = \begin{bmatrix}
\Gamma & \epsilon \\ \epsilon & 1
\end{bmatrix}    \begin{bmatrix} y_1 \\ y_2 \end{bmatrix} - \begin{bmatrix}
\Gamma & \epsilon \\ \epsilon & 1
\end{bmatrix} \begin{bmatrix} g(t)+ g'(t)\\ g(\omega t)+g'(\omega t) \end{bmatrix}. 
\end{equation}
we set $g(t) = \cos(t)$ with $\omega = 100, \Gamma = - 1/ \omega = -0.01 , \epsilon = 1/\omega = 0.01$.

\subsection{Reaction-Diffusion problem}
We consider a reaction-diffusion problem with a traveling wave solution.
\begin{equation}
u_t = \epsilon u_{xx} + \gamma u^2(1 - u),
\end{equation}
for $0<x<L, 0<t\leq T$. Initial and boundary conditions are given by
\begin{equation}
u_x(0,t) = u_x(L,t) = 0 , \hspace{9mm} u(x,0) = (1+ e^{\lambda(x-1)})^{-1},
\end{equation}
where $\lambda = \frac{1}{2} \sqrt{2 \gamma/\epsilon}$.
\subsection{Set up of test problems and results}
\underline{Things we are keeping track of:} 
\begin{itemize}
\item Max error
\item Time for evaluation
\item Number of function calls
\end{itemize}
\underline{Parameters we can change}
\begin{itemize}
\item $h$ values (make them smaller and smaller) (Which ones?)
\item $m$ values (increase value), this translates to a change in $h_{fast}$ (decrease value). (Which ones?) 
\item Inner ERK methods being used (Heun, ERK-3-3, ERK-4-4)
\end{itemize}

\underline{Questions:}
\begin{itemize}
\item What's the strategy for setting up these tests? Need to know what drivers to create and what information to set up to be stored in each case. 
\item Nail down time intervals to solve problems on
\end{itemize}
\end{document}
